\frac{dv}{dt} &=  -I_{Leak} - I_{Ca} - I_{Na}  - I_K\\
\frac{db}{dt} &= \frac{ b_{\infty}-b }{\tau_b} \\
\frac{dg}{dt} &= \frac{ g_{\infty}-g }{\tau_g} \\
\frac{dh}{dt} &= \frac{ h_{\infty}-h }{\tau_h} \\
\frac{dm}{dt} &= \frac{ m_{\infty}-m }{\tau_m} \\
\frac{dn}{dt} &= \frac{ n_{\infty}-n }{\tau_n} \\
\frac{dq}{dt} &= \frac{ q_{\infty}-q }{\tau_q} \\
I_{Leak} &= G_{Leak}( v-E_{Leak} ) \\
I_{Ca} &=  G_{Ca}b^2g^2( v-E_{Ca} ) \\
I_{Na} &= G_{Na}mh( v-E_{Na} ) \\
I_K &= G_Kn^2q^2( v-E_{K} ) \\
{\tau_b} &= \frac{s_{\tau_b}}{\exp\left (\frac{\theta_{\tau_b} - v}{\sigma^2_{\tau_b}}\right ) + \exp\left (-\frac{\theta_{\tau_b} - v}{\sigma^1_{\tau_b}}\right ) }\\
{\tau_g} &= \frac{s_{\tau_g}}{\exp\left (\frac{\theta_{\tau_g} - v}{\sigma^2_{\tau_g}}\right ) + \exp\left (-\frac{\theta_{\tau_g} - v}{\sigma^1_{\tau_g}}\right ) }\\
{\tau_h} &= \frac{s_{\tau_h}}{\exp\left (\frac{\theta_{\tau_h} - v}{\sigma^2_{\tau_h}}\right ) + \exp\left (-\frac{\theta_{\tau_h} - v}{\sigma^1_{\tau_h}}\right ) }\\
{\tau_m} &= \frac{s_{\tau_m}}{\exp\left (\frac{\theta_{\tau_m} - v}{\sigma^2_{\tau_m}}\right ) + \exp\left (-\frac{\theta_{\tau_m} - v}{\sigma^1_{\tau_m}}\right ) }\\
{\tau_n} &= \frac{s_{\tau_n}}{\exp\left (\frac{\theta_{\tau_n} - v}{\sigma^2_{\tau_n}}\right ) + \exp\left (-\frac{\theta_{\tau_n} - v}{\sigma^1_{\tau_n}}\right ) }\\
{\tau_q} &= \frac{s_{\tau_q}}{\exp\left (\frac{\theta_{\tau_q} - v}{\sigma^2_{\tau_q}}\right ) + \exp\left (-\frac{\theta_{\tau_q} - v}{\sigma^1_{\tau_q}}\right ) }\\
b_{\infty} &= \frac{1}{\exp\left (\frac{\theta_{b_{\infty}} - v}{\sigma_{b_{\infty}}}\right ) + 1 }\\
g_{\infty} &= \frac{1}{\exp\left (-\frac{\theta_{g_{\infty}} - v}{\sigma_{g_{\infty}}}\right ) + 1 }\\
h_{\infty} &= \frac{1}{\exp\left (-\frac{\theta_{h_{\infty}} - v}{\sigma_{h_{\infty}}}\right ) + 1 }\\
m_{\infty} &= \frac{1}{\exp\left (\frac{\theta_{m_{\infty}} - v}{\sigma_{m_{\infty}}}\right ) + 1 }\\
n_{\infty} &= \frac{1}{\exp\left (\frac{\theta_{n_{\infty}} - v}{\sigma_{n_{\infty}}}\right ) + 1 }\\
q_{\infty} &= \frac{1}{\exp\left (-\frac{\theta_{q_{\infty}} - v}{\sigma_{q_{\infty}}}\right ) + 1 }